% Created 2017-02-05 Sun 03:32
% Intended LaTeX compiler: pdflatex
\documentclass[11pt]{scrartcl}
  \usepackage[beaue, pset, anon]{masty}
\pSet{\hw{MAT247}{IV}{3}}
\pagenumbering{gobble}
\author{Alexander Illarionov}
\date{\today}
\title{}
\begin{document}

Suppose that \(V\) is a finite-dimensional inner product space and that
\(T : V \to V\) is a linear transformation.

\textbf{Problem}
Show that \(R(T^*)^\perp = \ker T\).

\textbf{Solution}

Note that for all \(x, y\in V\), \(\ipr{Tx}{y}= \ipr{x}{T^{*}y}\).

Therefore, if \(x\in\ker T\), then \(Tx = 0\). Therefore, from above,
\(\ipr{0}{y} = 0 = \ipr{x}{T^{*}y}\).

Note that \(T^{*}y \in \Img T^{*}\), and since \(y\) is arbitrary, it follows
that \(\ker T \suq (\Img T^{*})^{\perp}\).

Suppose now \(y\in (\Img T^{*})^{\perp}\). Therefore, for all \(u\in \Img T^{*}\),
\(\ipr{u}{y} =0\).

Fix some \(u\). Since \(u\in \Img T^{*}\), there exists \(x\in V\) such that
\(T^{*}x = u\).

Thus, \(\ipr{T^{*}x}{y} = 0 = \ipr{x}{Ty}\).

Since \(u\) was chosen arbitrarily, then this holds for any \(u\) and
 corresponding \(x\). Therefore \(Ty = 0\), and hence \((\Img
 T^{*})^{\perp}\suq \ker T\).

Therefore, \(R(T^*)^\perp = \ker T\).

\begin{lemma*}
\label{SEC:1}
For any finite dimensional vector space $V$, if $S\suq V$ and $S\neq \emptyset$, then $S=(S^{\bot})^{\bot}.
\end{lemma*}

\begin{proof}
\hfill

Note that $S^{\bot} = \set{x\in V: \forall y\in S.\ipr{x}{y} = 0}.

Therefore, $(S^{\bot})^{\bot} = \set{v\in V: \forall w\in S^{\bot}.\ipr{v}{w} = 0}.

Suppose $u\in S$ and $w\in S^{\bot}$. Since $\forall y\in S.\ipr{w}{y} = 0$, $\ipr{w}{u} = 0$.

Since $\ipr{w}{u} = \ol{\ipr{u}{w}}$ and $\ol{0} = 0$, then $\ipr{u}{w} = 0$. 

Since $w$ is arbitrary, $\forall w\in S^{\bot}. \ipr{u}{w} = 0$. Therefore, by definition, $u\in S^{\bot}^{\bot}$, and thus $S \suq S^{\bot\bot}.

Suppose now $s\in S^{\bot}^{\bot}$.

Therefore, $\forall w\in S^{\bot}$. Take some $w\in S^{\bot}$.

Note that $\ipr{s}{w} = 0$. Similarly to the argument given above, we can deduce that $\ipr{w}{s} = 0$.

Since $s$ is arbitrary, $\forall s\in S^{\bot\bot}. \ipr{s}{w}=0$. Therefore, by definition of $S^{\bot}$, it follows that $s\in S$, and hence $S\suq S^{\bot\bot}$. 
\end{proof}

From Lemma \ref{SEC:1} we obtain that \((\Img T^{*})^{\bot\bot} = \Img T^{*} = (\ker T)^{\bot}\).

Moreover, since \(T^{**} = T\), substituting \(T^{*}\), we get that \((\Img T)^{\bot} = \ker T^{*}\).

By the rank-nullity theorem, \(\nll T^{*} + \rank T^{*} = \dim V\). 

Since \(V = \Img T\oplus (\Img T)^{\bot}\), we also obtain that \(\dim V
= \rank T + \dim \Img T^{\bot}\).

Thus, 
\[\rank T + \dim \Img T^{\bot} = \nll T^{*} + \rank T^{*}\]

Since \((\Img T)^{\bot} = \ker T^{*}\), we get \(\dim (\Img T)^{*} = \nll
T^{*}\), and therefore, \(\rank T = \rank T^{*}\).
\end{document}